WIP

src/theories/RAs.v
@@ -6,21 +6,23 @@ Require Import lang.
 Section RA.
   (* Context{A V W R P F:Type} `{Countable A, Countable V, Countable W, Countable R, Countable P}. *)
 
-  Class gen_VMPreG (A V W R P F: Type) (Σ:gFunctors) `{Countable A, Countable V, Countable W, Countable R, Countable P} := {
+  Class gen_VMPreG (A V W R P F: Type) (Σ:gFunctors)
+        `{Countable A, Countable V, Countable W, Countable R, Countable P} := {
                       gen_num_preG_inG :> inG Σ (agreeR natO);
                       gen_mem_preG_inG :> gen_heapPreG A W Σ;
                       gen_reg_preG_inG :> gen_heapPreG (R * V) W Σ;
                       gen_tx_preG_inG :> inG Σ (authR (gmapUR V (agreeR (leibnizO P))));
-                      gen_rx_preG_inG :> inG Σ (prodR (authR (gmapUR V (agreeR (leibnizO P)))) (optionR (gmap_viewR V (prodO boolO (prodO natO (leibnizO V))))));
-                      gen_owned_preG_inG :> inG Σ (authR (gset_disjUR P));
+                      gen_rx_preG_inG :> inG Σ (prodR (authR (gmapUR V (agreeR (leibnizO P))))
+                                                      (optionR (gmap_viewR V (optionO (prodO natO (leibnizO V))))));
+                      gen_owned_preG_inG :> inG Σ (authR (gset_disjUR (leibnizO P)));
                       gen_access_preG_inG :> inG Σ (authR (gmapUR P (prodR dfracR (csumR (agreeR unitO) (exclR unitO)))));
                       gen_trans_preG_inG :> gen_heapPreG W (V * W* W*(gmap V (gset P))*F) Σ;
                       gen_retri_preG_inG :> inG Σ (authR (gmapUR W (gset_disjR (leibnizO V))))
                    }.
 
 
- Class gen_VMG(A V W R P F: Type) Σ `{Countable A, Countable V, Countable W, Countable R, Countable P}  := GenVMG{
-                      gen_VM_inG :> gen_VMPreG A V W R P F Σ;
+ Class gen_VMG Σ := GenVMG{
+                      gen_VM_inG :> gen_VMPreG Addr VMID Word RegName PID HvcFunc  Σ;
                       gen_num_name : gname;
                       gen_mem_name : gname;
                       gen_reg_name : gname;
@@ -32,45 +34,107 @@ Section RA.
                       gen_retri_name : gname
                     }.
 
+Global Arguments gen_num_name {Σ} _.
+Global Arguments gen_mem_name {Σ} _.
+Global Arguments gen_reg_name {Σ} _.
+Global Arguments gen_rx_name {Σ} _.
+Global Arguments gen_tx_name {Σ} _.
+Global Arguments gen_owned_name {Σ} _.
+Global Arguments gen_access_name {Σ} _.
+Global Arguments gen_trans_name {Σ} _.
+Global Arguments gen_retri_name {Σ} _.
 
-Global Arguments GenVMG A V W R P F Σ {_ _ _ _ _ _ _ _ _ _ _ } _ _ _ _ _ _ _ _ _.
-Global Arguments gen_num_name {A V W R P F Σ _ _ _ _ _ _ _ _ _ _ } _.
-Global Arguments gen_mem_name {A V W R P F Σ _ _ _ _ _ _ _ _ _ _ } _.
-Global Arguments gen_reg_name {A V W R P F Σ _ _ _ _ _ _ _ _ _ _ } _.
-Global Arguments gen_rx_name {A V W R P F Σ _ _ _ _ _ _ _ _ _ _ } _.
-Global Arguments gen_tx_name {A V W R P F Σ _ _ _ _ _ _ _ _ _ _ } _.
-Global Arguments gen_owned_name {A V W R P F Σ _ _ _ _ _ _ _ _ _ _ } _.
-Global Arguments gen_access_name {A V W R P F Σ _ _ _ _ _ _ _ _ _ _ } _.
-Global Arguments gen_trans_name {A V W R P F Σ _ _ _ _ _ _ _ _ _ _ } _.
-Global Arguments gen_retri_name {A V W R P F Σ _ _ _ _ _ _ _ _ _ _ } _.
+Definition ra_TXBuffer :=
+  (authR (gmapUR VMID (agreeR (leibnizO PID)))).
 
-Definition gen_VMΣ (A V W R P F: Type) `{Countable A, Countable V, Countable W, Countable R, Countable P} : gFunctors :=
+Definition ra_RXBuffer :=
+  (prodR ra_TXBuffer
+         (optionR (gmap_viewR VMID (optionO (prodO natO (leibnizO VMID)))))).
+Definition ra_Accessible:=
+  (authR (gmapUR PID (prodR dfracR (csumR (agreeR unitO) (exclR unitO))))).
+
+
+Definition gen_VMΣ : gFunctors :=
   #[
       GFunctor (agreeR natO);
-      gen_heapΣ A W;
-      gen_heapΣ (R * V) W;
-      GFunctor (authR (gmapUR V (agreeR (leibnizO P))));
-      GFunctor (prodR (authR (gmapUR V (agreeR (leibnizO P)))) (optionR (gmap_viewR V (prodO boolO (prodO natO (leibnizO V))))));
-      GFunctor (authR (gset_disjUR P));
-      GFunctor (authR (gmapUR P (prodR dfracR (csumR (agreeR unitO) (exclR unitO)))));
-      gen_heapΣ W (V * W * W * (gmap V (gset P)) *F);
-      GFunctor (authR (gmapUR W (gset_disjR (leibnizO V))))
+      gen_heapΣ Addr Word;
+      gen_heapΣ (RegName * VMID) Word;
+      GFunctor ra_TXBuffer;
+      GFunctor ra_RXBuffer;
+      GFunctor (authR (gset_disjUR (leibnizO PID)));
+      GFunctor ra_Accessible;
+      gen_heapΣ Word (VMID * Word * Word * (gmap VMID (gset PID)) * HvcFunc);
+      GFunctor (authR (gmapUR Word (gset_disjR (leibnizO VMID))))
    ].
 
-Global Instance subG_gen_VMPreG {Σ A V W R P F} `{Countable A, Countable V, Countable W, Countable R, Countable P}:
-  subG (gen_VMΣ A V W R P F) Σ -> gen_VMPreG A V W R P F Σ.
+Global Instance subG_gen_VMPreG {Σ}:
+  subG gen_VMΣ Σ -> gen_VMPreG Addr VMID Word RegName PID HvcFunc Σ.
 Proof.
   (* hack: solve_inG does not currently unfold [subG X _] where X has more than
      4 parameters. We have 6 (A, V, W, R, P, F). *)
-  set HA := gen_VMΣ A V W R P F. unfold gen_VMΣ in HA.
+  (* set HA := gen_VMΣ. unfold gen_VMΣ in HA. *)
   solve_inG.
 Qed.
 
 Section definitions.
-  Context `{Countable A, Countable V, Countable W, Countable RG, Countable P,
-            vmG : !gen_VMG A V W RG P F Σ}.
+  Context `{vmG : !gen_VMG Σ}.
+  Implicit Type σ: State.
+  Implicit Type δ: VMState.
 
-  Definition gen_vm_interp (σ: State) : iProp Σ :=
-    own (gen_num_name vmG) (to_agree (map_size (vmStates σ))) ∗
-    ghost_map_auth (gen_mem_name vmG) 1 (mem σ).
-  .
+  Definition get_reg_gmap δ (i: VMID): gmap (RegName * VMID) Word :=
+    list_to_map (map  (λ (p: RegName * Word), ((p.1 , i), p.2))
+                      (map_to_list (δ.1.1))).
+
+  Definition get_txrx_auth_agree σ (f: MailBox -> PID) :
+    ra_TXBuffer:=
+    (● ((λ (δ: VMState), to_agree (f δ.1.2)) <$> (vmStates σ))).
+
+  Definition get_rx_state δ :(optionO (prodO natO (leibnizO VMID))):=
+    let mb := δ.1.2 in
+    match mb.2.2 with
+      | Some j => (Some (0, j))
+      | None => None
+    end.
+   (* HACK : don't know why *)
+   (* match perm.1 with *)
+   (*                | Owned => s ⊎ {[ p ]} *)
+   (*                | Unowned => s *)
+   (*               end ) *)
+   (* doesn't work...*)
+  Definition get_owned_gset δ : (authR (gset_disjUR PID)) :=
+    (● (map_fold (λ (p:PID) (perm:Perm) (s: gset_disjUR PID),
+                  match perm.1 with
+                  | Owned =>  match s with
+                                | GSet s' => GSet (s' ∪ {[p]})
+                                | GSetBot => GSet ∅
+                              end
+                  | Unowned => s
+                 end)  (GSet ∅)  δ.2 )).
+
+  Definition get_access_gmap δ : ra_Accessible :=
+    (●  (map_fold (λ (p:PID) (perm:Perm) (s: (gmap PID (prodR dfracR (csumR (agreeR unitO) (exclR unitO))))),
+                  match perm.2 with
+                  | NoAccess => s
+                  | SharedAccess => <[p:= ((DfracOwn 1), (Cinl (to_agree ())))]>s
+                  | ExclusiveAccess => <[p:= ((DfracOwn 1),(Cinr (Excl ())))]>s
+                 end)  ∅  δ.2 )).
+
+  (* TODO *)
+  Definition get_trans_gmap σ : gmap Word (VMID * Word * Word * (gmap VMID (gset PID)) * HvcFunc).
+
+
+  Definition gen_vm_interp σ: iProp Σ :=
+    let n := (map_size (vmStates σ)) in
+    let i := (currentVM σ) in
+    match (vmState σ i) with
+    | Some δ =>  own (gen_num_name vmG) (to_agree n) ∗
+                 ghost_map_auth (gen_mem_name vmG) 1 (mem σ) ∗
+                 ghost_map_auth (gen_reg_name vmG) 1 (get_reg_gmap δ i) ∗
+                 own (gen_tx_name vmG) (get_txrx_auth_agree σ (λ p, p.1)) ∗
+                 own (gen_rx_name vmG) ((get_txrx_auth_agree σ (λ p, p.2.1)),
+                                        (Some (gmap_view_auth 1 ((get_rx_state) <$> (vmStates σ))))) ∗
+                 own (gen_owned_name vmG) (get_owned_gset δ) ∗
+                 own (gen_access_name vmG) (get_access_gmap δ) ∗
+                 ghost_map_auth (gen_trans_name vmG) 1 (get_trans_gmap σ)
+    | None => True
+    end.
